

CHAIN RULE - EXAMPLES

CHAIN RULE:

$$\text{If } g(x) = (f(x))^n$$

$$\text{then } g'(x) = n(f(x))^{n-1} \times f'(x)$$

with high n
and two or
more terms in
the bracket

REVERSE CHAIN RULE:

$$\text{If } f(x) = (f(x))^n$$

$$\text{then } F(x) = \frac{(f(x))^{n+1}}{(n+1) \times (f'(x))}$$

Capital F for integral
of f

EXAMPLES $f(x) =$ the following

- A
- ① $(x+2)^2$
 - ② $(2x+3)^4$
 - ③ $(x^3+4)^5$
 - ④ $(3x+2)^{-1}$

What is $f'(x)$ in each case?

- ⑤ $\frac{1}{(x^2-3)^3}$
- ⑥ $(x^2-1)^{\frac{3}{2}}$
- ⑦ $\left(\frac{1}{x}+x\right)^3$
- ⑧ $4(x+2)^2$

$f(x) =$ the following

What is $F(x)$ in each case
(integrate the following)

- B
- ① $2(x+2)$
 - ② $8(2x+3)^3$
 - ③ $15x^2(x^3+4)^4$
 - ④ $\frac{-3}{(3x+2)^2}$

- ⑤ $\frac{-6x}{(x^2-3)^4}$
- ⑥ $3x(x^2-1)^{\frac{1}{2}}$
- ⑦ $3\left(\frac{1}{x}+x\right)^2\left(-\frac{1}{x^2}+1\right)$
- ⑧ $8(x+2)$

ANSWERS

$$A \text{ (1)} \quad f(x) = (x+2)^2$$

$$f'(x) = 2(x+2) \times 1 \\ = 2(x+2)$$

$$\text{(2)} \quad f(x) = (2x+3)^4$$

$$f'(x) = 4(2x+3)^3 \times 2 \\ = 8(2x+3)^3$$

$$\text{(3)} \quad f(x) = (x^3+4)^5$$

$$f'(x) = 5(x^3+4)^4 \times 3x^2 \\ = 15x^2 (x^3+4)^4$$

$$\text{(4)} \quad f(x) = (3x+2)^{-1}$$

$$f'(x) = -1(3x+2)^{-2} \times 3 \\ = -3(3x+2)^{-2} \\ = \frac{-3}{(3x+2)^2}$$

$$\text{(5)} \quad f(x) = \frac{1}{(x^2-3)^3}$$

$$f'(x) = -3(x^2-3)^{-4} \times 2x \\ = -6x(x^2-3)^{-4} \\ = \frac{-6x}{(x^2-3)^4}$$

$$\textcircled{6} \quad f(x) = (x^2 - 1)^{\frac{3}{2}}$$

$$\begin{aligned} f'(x) &= \frac{3}{2} (x^2 - 1)^{\frac{1}{2}} \times 2x \\ &= 3x (x^2 - 1)^{\frac{1}{2}} \end{aligned}$$

$$\textcircled{7} \quad f(x) = \left(\frac{1}{x} + x\right)^3$$

$$\begin{aligned} f'(x) &= 3 \left(\frac{1}{x} + x\right)^2 \times \left(-x^{-2} + 1\right) \\ &= 3 \left(\frac{1}{x} + x\right)^2 \left(-\frac{1}{x^2} + 1\right) \end{aligned}$$

$$\textcircled{8} \quad f(x) = 4(x+2)^2$$

$$\begin{aligned} f'(x) &= 8(x+2) \times 1 \\ &= 8(x+2) \end{aligned}$$

$$\text{B } \textcircled{1} \quad f(x) = 2(x+2)$$

$$F(x) = \frac{2(x+2)^2}{2 \times 1}$$

$$= \frac{2(x+2)^2}{2}$$

$$= (x+2)^2$$

$$\textcircled{2} \quad f(x) = 8(2x+3)^3$$

$$F(x) = \frac{8(2x+3)^4}{4 \times 2}$$

$$= \frac{8(2x+3)^4}{8}$$

$$= (2x+3)^4$$

$$\textcircled{3} \quad f(x) = 15x^2(x^3+4)^4$$

$$F(x) = \frac{15x^2(x^3+4)^5}{5 \times 3x^2}$$

$$= \frac{15x^2(x^3+4)^5}{15x^2}$$

$$= (x^3+4)^5$$

$$\textcircled{4} \quad f(x) = \frac{-3}{(3x+2)^2}$$

$$F(x) = \frac{-3(3x+2)^{-1}}{-1 \times 3}$$

$$= (3x+2)^{-1}$$

$$= \frac{1}{3x+2}$$

$$\textcircled{5} \quad f(x) = \frac{-6x}{(x^2-3)^4}$$

6

$$F(x) = \frac{-6x(x^2-3)^{-3}}{-3 \times 2x}$$

$$= (x^2-3)^{-3}$$

$$= \frac{1}{(x^2-3)^3}$$

$$\textcircled{6} \quad f(x) = 3x(x^2-1)^{\frac{1}{2}}$$

$$F(x) = \frac{3x(x^2-1)^{\frac{3}{2}}}{\frac{3}{2} \times 2x}$$

$$= 3x(x^2-1)^{\frac{3}{2}}$$

$$= (x^2-1)^{\frac{3}{2}}$$

$$\textcircled{7} \quad f(x) = 3\left(\frac{1}{x}+x\right)^2\left(-\frac{1}{x^2}+1\right)$$

$$F(x) = \frac{\cancel{3}x\left(-\frac{1}{x^2}+1\right) \times \left(\frac{1}{x}+x\right)^3}{\cancel{3} \times \left(-\frac{1}{x^2}+1\right)}$$

$$F(x) = \left(\frac{1}{x}+x\right)^3$$

$$\textcircled{8} \quad f(x) = 8(x+2)$$

$$F(x) = \frac{8(x+2)^2}{2 \times 1}$$

$$= 4(x+2)^2$$